hol/symb_exec/symb_execLib.sig
@@ -2,7 +2,7 @@ signature symb_execLib =
 sig
   include Abbrev
 
-datatype path_tree = empty | node of int * thm * (path_tree list);
+datatype path_tree = empty | node of int * term * thm * (path_tree list);
 
 val symb_exec:
  (thm * thm -> thm) * thm * (thm -> (term list * thm) option) *
